\documentclass{article}
\usepackage{amsmath}
\title{Force calculations with PIMC}
\author{Kenneth P. Esler Jr.}
\date{\today}

\newcommand{\vr}{\mathbf{r}}
\newcommand{\vrp}{\mathbf{r}'}
\newcommand{\vR}{\mathbf{R}}


\begin{document}
\maketitle

\section{Introduction}

\section{Pair action gradients}

\begin{eqnarray}
\vr \equiv   \vr_\text{elec} - \vR \\
\vrp \equiv  \vrp_\text{elec} - \vR
\end{eqnarray}
Now $u = u(\vr,\vrp;\tau)$.  We wish to compute the gradient,
$\nabla_\vR u(\vr, \vrp; \tau)$.  Because of symmetry, it is
convenient to store, $u(\vr, \vrp;\tau) = u(q,s,z)$, where
\begin{eqnarray}
q \equiv \frac{|\vr| + |\vrp|}{2} \\
z \equiv \frac{|\vr| - |\vrp|}{2} \\
s \equiv |\vr - \vrp|
\end{eqnarray}
Since $s$ is independent of $\vR$, we may write
\begin{equation}
\nabla_\vR u = \frac{\partial u}{\partial q} \nabla_\vR q +
\frac{\partial u}{\partial z} \nabla_\vR z
\end{equation}
Then we may write
\begin{eqnarray}
q & = & \frac{1}{2} \left\{\left[ (R_x - r_x)^2 + (R_y - r_y)^2 +
  (R_z-r_z)^2\right]^{\frac{1}{2}}+ 
\left[(R_x-r'_x)^2 +(R_y-r'_y)^2 +
  (R_z-r'_z)^2\right]^\frac{1}{2}\right\} \\
z & = &\frac{1}{2} \left\{\left[ (R_x - r_x)^2 + (R_y - r_y)^2 +
  (R_z-r_z)^2\right]^{\frac{1}{2}}- 
\left[(R_x-r'_x)^2 +(R_y-r'_y)^2 +
  (R_z-r'_z)^2\right]^\frac{1}{2}\right\} 
\end{eqnarray}
Hence,
\begin{eqnarray}
  \nabla_\vR q & = & -\frac{\hat{\vr} + \hat{\vr}'}{2} \\
  \nabla_\vR z & = & -\frac{\hat{\vr} - \hat{\vr}'}{2} \\
\end{eqnarray}
Then, we have
\begin{equation}
\nabla_{\vR} u(q,z,s;\tau) = -\frac{1}{2}\left[\frac{\partial u}{\partial q}
\left(\hat{\vr} + \hat{\vr}'\right)
-\frac{\partial u}{\partial z} \left(\hat{\vr} -\hat{\vr}'\right) \right]
\end{equation}



\end{document}
